proofs for String_Shenanigans.thy, progress on Precondition Normalization

Precondition_Normalization.thy
@@ -1,12 +1,8 @@
 theory Precondition_Normalization
 imports "AI_Planning_Languages_Semantics.PDDL_STRIPS_Semantics"
-    String_Shenanigans PDDL_Sema_Supplement DNF
+    PDDL_Sema_Supplement Utils String_Shenanigans DNF
 begin
 
-(*
-This part helps ensure that names of the split actions are unique.
-This part calculates the DNF for every precondition, only to then discard them again,
-before they are later recalculated... TODO This should probably be cached using Let. *)
 definition "n_clauses ac \<equiv> length (dnf_list (ast_action_schema.precondition ac))"
 
 context ast_domain begin
@@ -14,16 +10,14 @@ context ast_domain begin
 definition "max_n_clauses \<equiv> Max (set (map n_clauses (actions D)))"
 definition "prefix_padding \<equiv> max_length (distinct_strings max_n_clauses) + 1"
 
-fun (in -)set_n_pre :: " ast_action_schema \<Rightarrow> string \<Rightarrow> term atom formula \<Rightarrow> ast_action_schema" where
+fun (in -) set_n_pre :: " ast_action_schema \<Rightarrow> string \<Rightarrow> term atom formula \<Rightarrow> ast_action_schema" where
   "set_n_pre (Action_Schema _ params _ eff) n pre
   = Action_Schema n params pre eff"
-
 
 definition "split_ac_names ac n \<equiv>
   map (\<lambda>prefix. pad prefix_padding prefix @ ac_name ac) (distinct_strings n)"
 
-
-fun split_ac :: "ast_action_schema \<Rightarrow> ast_action_schema list" where
+definition split_ac :: "ast_action_schema \<Rightarrow> ast_action_schema list" where
   "split_ac ac =
     (let clauses = dnf_list (ac_pre ac) in
     map2 (set_n_pre ac) (split_ac_names ac (length clauses)) clauses)"
@@ -44,14 +38,104 @@ definition (in ast_problem) "split_prob \<equiv>
     (init P)
     (goal P)"
 
-
 (* it's important to be able to convert a plan for the output problem into a plan for the input problem.
   The other direction is probably (hopefully?) not important. *)
-
 fun restore_pa_split where
   "restore_pa_split (PAction n args) = PAction (drop prefix_padding n) args"
 abbreviation "restore_plan_split \<pi>s \<equiv> map restore_pa_split \<pi>s"
 
+definition (in ast_domain) "precond_normed_dom \<equiv>
+  \<forall>ac \<in> set (actions D). is_conj (ac_pre ac)"
+
+definition (in ast_problem) "precond_normed_prob \<equiv> precond_normed_dom"
+
+end
+
+section \<open> Precondition Normalization Proofs \<close>
+
+text \<open> locale setup for simplified syntax \<close>
+
+abbreviation (in ast_domain) (input) "D4 \<equiv> split_dom"
+abbreviation (in ast_problem) (input) "P4 \<equiv> split_prob"
+
+locale ast_domain4 = ast_domain
+sublocale ast_domain4 \<subseteq> d4: ast_domain D4 .
+
+locale wf_ast_domain4 = wf_ast_domain
+sublocale wf_ast_domain4 \<subseteq> d4: ast_domain D4 .
+sublocale wf_ast_domain4 \<subseteq> ast_domain4 .
+
+locale ast_problem4 = ast_problem
+sublocale ast_problem4 \<subseteq> p4: ast_problem P4 .
+sublocale ast_problem4 \<subseteq> ast_domain4 D .
+
+locale wf_ast_problem4 = wf_ast_problem
+sublocale wf_ast_problem4 \<subseteq> p4 : ast_problem P4.
+sublocale wf_ast_problem4 \<subseteq> ast_problem4 .
+sublocale wf_ast_problem4 \<subseteq> wf_ast_domain4 D
+  by unfold_locales
+
+text \<open> Alternate definitions \<close>
+
+(* probably unnecessary *)
+lemma set_n_pre_alt: "set_n_pre ac n pre =
+  Action_Schema n (ac_params ac) pre (ac_eff ac)"
+  by (cases ac) simp
+
+(* probably unnecessary *)
+lemma set_n_pre_sel [simp]:
+  "ac_name (set_n_pre ac n pre) = n"
+  "ac_params (set_n_pre ac n pre) = ac_params ac"
+  "ac_pre (set_n_pre ac n pre) = pre"
+  "ac_eff (set_n_pre ac n pre) = ac_eff ac"
+  using set_n_pre_alt by simp_all
+
+thm ast_domain.split_ac_def
+
+lemma
+  "i < length as \<Longrightarrow> i < length bs \<Longrightarrow> map2 f as bs ! i = f (as!i) (bs!i)"
+  by simp
+
+lemma (in ast_domain)
+  assumes "i < length (dnf_list (ac_pre ac))"
+  shows "split_ac ac ! i =
+    set_n_pre ac
+    ((\<lambda>prefix. pad prefix_padding prefix @ ac_name ac) (distinct_strings (length (dnf_list (ac_pre ac))) ! i))
+    (dnf_list (ac_pre ac) ! i)"
+  using assms unfolding split_ac_def split_ac_names_def set_n_pre_alt Let_def sorry
+
+lemma (in ast_domain) split_dom_sel [simp]:
+  "types D4 = types D"
+  "predicates D4 = predicates D"
+  "consts D4 = consts D"
+  "actions D4 = split_acs"
+  using split_dom_def by simp_all
+
+lemma (in ast_problem) split_prob_sel [simp]:
+  "domain P4 = D4"
+  "objects P4 = objects P"
+  "init P4 = init P"
+  "goal P4 = goal P"
+  using split_prob_def by simp_all
+
+
+subsection \<open> Output format \<close>
+
+context ast_problem4 begin
+thm precond_normed_dom_def
+(* \<forall>ac \<in> set (actions D). is_conj (ac_pre ac) *)
+
+thm split_ac_def
+lemma prec_normed_ac:
+  "\<forall>ac' \<in> set (split_ac ac). is_conj (ac_pre ac')"
+proof -
+  have "\<forall>c \<in> set (dnf_list (ac_pre ac)). is_conj c"
+    using dnf_list_conjs by auto
+  have "\<forall>ac' \<in> set (split_ac ac). ac_pre ac \<in>
+    set (dnf_list (ac_pre ac))" unfolding split_ac_def Let_def sorry
+  thus ?thesis
+    unfolding split_ac_def Let_def sorry
+qed
 
 end
 
@@ -62,7 +146,7 @@ lemmas precond_norm_code =
   ast_domain.max_n_clauses_def
   ast_domain.prefix_padding_def
   ast_domain.split_ac_names_def
-  ast_domain.split_ac.simps
+  ast_domain.split_ac_def
   ast_domain.split_acs_def
   ast_domain.split_dom_def
   ast_problem.split_prob_def
