String_Shenanigans.thy
@@ -61,28 +61,76 @@ qed
 definition pad_strings :: "string list \<Rightarrow> string list" where
   "pad_strings ss \<equiv> map (pad (max_length ss + 1)) ss"
 
-lemma
-  assumes "distinct xs"
-    "\<forall>y \<in> set ys. length y = n"
-  shows "distinct (map2 (@) ys xs)"
-  using assms oops
+fun nat_upto_help :: "nat \<Rightarrow> nat list \<Rightarrow> nat list" where
+  "nat_upto_help 0 build = 0 # build" |
+  "nat_upto_help (Suc n) build = nat_upto_help n (Suc n # build)"
+
+definition "nat_upto n \<equiv> nat_upto_help n []"
+
+lemma nat_upto_help_length: "length (nat_upto_help n xs) = n + 1 + length xs"
+  by (induction n arbitrary: xs) simp_all
+
+lemma nat_upto_length [simp]: "length (nat_upto n) = n + 1"
+  unfolding nat_upto_def using nat_upto_help_length by simp
+
+lemma nat_upto_help_aux: "nat_upto_help n (xs@ys) = nat_upto_help n xs @ ys"
+proof (induction n arbitrary: xs)
+  case (Suc n)
+  have "nat_upto_help (Suc n) (xs @ ys) = nat_upto_help n ((Suc n # xs) @ ys)" by simp
+  also have "... = nat_upto_help n (Suc n # xs) @ ys" using Suc.IH by blast
+  also have "... = nat_upto_help (Suc n) xs @ ys" by simp
+  finally show ?case by simp
+qed simp
+
+lemma "(xs @ [y]) ! length xs = y" by simp
+
+lemma nat_upto_help_nth: assumes "i \<le> n" shows "nat_upto_help n xs ! i = i"
+using assms proof (induction n arbitrary: i xs)
+  case (Suc n)
+  then consider "i \<le> n" | "i = Suc n" using le_SucE by blast
+  thus ?case
+  proof (cases)
+    case 2
+    have "nat_upto_help (Suc n) xs = nat_upto_help n ([] @ (Suc n # xs))" by simp
+    also have "... = nat_upto_help n [] @ (Suc n # xs)" using nat_upto_help_aux by metis
+    finally have "nat_upto_help (Suc n) xs ! i = (nat_upto_help n [] @ (Suc n # xs)) ! (length (nat_upto_help n []))"
+      using 2 nat_upto_help_length by simp
+    thus ?thesis using 2 by simp
+  qed (simp add: Suc)
+qed simp
+
+lemma nat_upto_nth [simp]: assumes "i \<le> n" shows "nat_upto n ! i = i"
+  using assms nat_upto_help_nth nat_upto_def by simp
+
+lemma nat_upto_distinct: "distinct (nat_upto n)"
+proof -
+  have "nat_upto n ! i \<noteq> nat_upto n ! j" if "i \<noteq> j" "i \<le> n" "j \<le> n" for i j
+    using nat_upto_nth that by simp
+  moreover have "i \<le> n \<longleftrightarrow> i < length (nat_upto n)" for i by auto
+  ultimately show ?thesis using distinct_conv_nth by blast
+qed
+
+definition "unique_string (i::nat) \<equiv> show i"
+definition "distinct_strings n \<equiv> map unique_string (case n of 0 \<Rightarrow> [] | Suc m \<Rightarrow> nat_upto m)"
 
 lemma show_nat_inj: fixes a :: nat and b :: nat assumes "a \<noteq> b" shows "show a \<noteq> show b"
   using assms sorry
 
-fun nat_upto :: "nat \<Rightarrow> nat list" where
-  "nat_upto 0 = [0]" |
-  "nat_upto (Suc n) = Suc n # nat_upto n"
+lemma unique_str_bij:
+  "i \<noteq> j \<longleftrightarrow> unique_string i \<noteq> unique_string j"
+  using unique_string_def show_nat_inj by auto
 
-definition "distinct_strings n \<equiv> map show (case n of 0 \<Rightarrow> [] | Suc m \<Rightarrow> nat_upto m)"
+lemma distinct_str_length [simp]: "length (distinct_strings n) = n"
+  unfolding distinct_strings_def
+  by (cases n) simp_all
 
+lemma distinct_strings_nth [simp]:
+  assumes "i < n" shows "distinct_strings n ! i = unique_string i"
+  unfolding distinct_strings_def using assms by (cases n) simp_all
 
-
-
-lemma dist_str_props:
-  "length (distinct_strings n) = n"
+lemma distinct_strings_dist:
   "distinct (distinct_strings n)"
-  sorry
+  using unique_str_bij distinct_conv_nth by fastforce
 
 
 definition distinctize :: "string list \<Rightarrow> string list \<Rightarrow> string list" where
